pulse/pulse2rust/dpe/src/evercrypt_ed25519.rs
@@ -1,4 +1,4 @@
-pub fn sign (
+pub fn sign(
     signature: &mut [u8],
     p_private_key: (),
     v_private_key: (),
@@ -6,12 +6,19 @@ pub fn sign (
     msg_len: u32,
     p_msg: (),
     v_msg: (),
-    msg: &mut [u8]
-) { unsafe {
-  super::evercrypt::EverCrypt_Ed25519_sign(signature.as_mut_ptr(), private_key.as_mut_ptr(), msg_len, msg.as_mut_ptr());
-}}
+    msg: &mut [u8],
+) {
+    unsafe {
+        super::evercrypt::EverCrypt_Ed25519_sign(
+            signature.as_mut_ptr(),
+            private_key.as_mut_ptr(),
+            msg_len,
+            msg.as_mut_ptr(),
+        );
+    }
+}
 
-pub fn verify (
+pub fn verify(
     p_public_key: (),
     v_public_key: (),
     public_key: &mut [u8],
@@ -21,7 +28,14 @@ pub fn verify (
     msg: &mut [u8],
     p_signature: (),
     v_signature: (),
-    signature: &mut [u8]
-) -> bool { unsafe {
-  return super::evercrypt::EverCrypt_Ed25519_verify(public_key.as_mut_ptr(), msg_len, msg.as_mut_ptr(), signature.as_mut_ptr());
-}}
+    signature: &mut [u8],
+) -> bool {
+    unsafe {
+        return super::evercrypt::EverCrypt_Ed25519_verify(
+            public_key.as_mut_ptr(),
+            msg_len,
+            msg.as_mut_ptr(),
+            signature.as_mut_ptr(),
+        );
+    }
+}
